theories/rules/rules_AddSubLt.v
@@ -49,7 +49,6 @@ Section cap_lang_rules.
       z_of_argument regs rv1 = Some n1 ->
       z_of_argument regs rv2 = Some n2 ->
       incrementPC (<[ dst := WInt (denote i n1 n2) ]> regs) = None ->
-      regs' = (<[ dst := WInt (denote i n1 n2) ]> regs) ->
       AddSubLt_failure i regs dst rv1 rv2 regs'.
 
   Inductive AddSubLt_spec (i: instr) (regs: Reg) (dst: RegName) (rv1 rv2: Z + RegName) (regs': Reg): cap_lang.val -> Prop :=
@@ -92,6 +91,7 @@ Section cap_lang_rules.
     iNext. iIntros (e2 σ2 efs Hpstep).
     apply prim_step_exec_inv in Hpstep as (-> & -> & (c & -> & Hstep)).
     iSplitR; auto. eapply step_exec_inv in Hstep; eauto.
+    unfold exec in Hstep.
 
     specialize (indom_regs_incl _ _ _ Dregs Hregs) as Hri.
     erewrite regs_of_is_AddSubLt in Hri, Dregs; eauto.
@@ -107,6 +107,7 @@ Section cap_lang_rules.
       { destruct_or! Hinstr; rewrite Hinstr /= in Hstep.
         all: rewrite /RegLocate Hr0 in Hstep. all: repeat case_match; simplify_eq; eauto. }
       iFail "Hφ" AddSubLt_fail_nonconst1. }
+    apply (z_of_arg_mono _ r) in Hn1; auto.
 
     destruct (z_of_argument regs arg2) as [n2|] eqn:Hn2;
       pose proof Hn2 as Hn2'; cycle 1.
@@ -115,17 +116,15 @@ Section cap_lang_rules.
       destruct (Hri r0) as [r0v [Hr'0 Hr0]]. by unfold regs_of_argument; set_solver+.
       rewrite Hr'0 in Hn2. destruct r0v as [| ? ? ? ? ]; [ congruence |].
       assert (c = Failed ∧ σ2 = (r, m)) as (-> & ->).
-      { destruct_or! Hinstr; rewrite Hinstr /= in Hstep.
+      { destruct_or! Hinstr; rewrite Hinstr /= Hn1 in Hstep; cbn in Hstep.
         all: rewrite /RegLocate Hr0 in Hstep. all: repeat case_match; simplify_eq; eauto. }
       iFail "Hφ" AddSubLt_fail_nonconst2. }
+    apply (z_of_arg_mono _ r) in Hn2; auto.
 
-    eapply z_of_argument_Some_inv' in Hn1; eapply z_of_argument_Some_inv' in Hn2; eauto.
-
-    assert ((c, σ2) = updatePC (update_reg (r, m) dst (WInt (denote i n1 n2)))) as HH.
-    { destruct Hn1 as [ -> | (r1 & -> & _ & Hr1) ]; destruct Hn2 as [ -> | (r2 & -> & _ & Hr2) ].
-      all: destruct_or! Hinstr; rewrite Hinstr /= /RegLocate /update_reg /= in Hstep |- *; auto.
-      all: rewrite ?Hr1 ?Hr2 /= in Hstep; auto. }
-    rewrite /update_reg /= in HH.
+    assert (exec_opt i (r, m) = updatePC (update_reg (r, m) dst (WInt (denote i n1 n2)))) as HH.
+    { all: destruct_or! Hinstr; rewrite Hinstr /= /RegLocate /update_reg /= in Hstep |- *; auto.
+      all: by rewrite Hn1 Hn2; cbn. }
+    rewrite HH in Hstep. rewrite /update_reg /= in Hstep.
 
     destruct (incrementPC (<[ dst := WInt (denote i n1 n2) ]> regs))
       as [regs'|] eqn:Hregs'; pose proof Hregs' as H'regs'; cycle 1.
@@ -135,14 +134,15 @@ Section cap_lang_rules.
       2: by apply lookup_insert_is_Some'; eauto.
       2: by apply insert_mono; eauto.
       simplify_pair_eq.
-      iMod ((gen_heap_update_inSepM _ _ dst) with "Hr Hmap") as "[Hr Hmap]"; eauto.
+      rewrite Hregs' in Hstep. inversion Hstep.
       iFail "Hφ" AddSubLt_fail_incrPC. }
+
 
     (* Success *)
 
     eapply (incrementPC_success_updatePC _ m) in Hregs'
       as (p' & g' & b' & e' & a'' & a_pc' & HPC'' & HuPC & ->).
-    eapply updatePC_success_incl with (m':=m) in HuPC. 2: by eapply insert_mono; eauto.
+    eapply updatePC_success_incl with (m':=m) in HuPC. 2: by eapply insert_mono; eauto. rewrite HuPC in Hstep.
     simplify_pair_eq. iFrame.
     iMod ((gen_heap_update_inSepM _ _ dst) with "Hr Hmap") as "[Hr Hmap]"; eauto.
     iMod ((gen_heap_update_inSepM _ _ PC) with "Hr Hmap") as "[Hr Hmap]"; eauto.
