theories/rules/rules_IsPtr.v
@@ -53,14 +53,15 @@ Section cap_lang_rules.
     iNext. iIntros (e2 σ2 efs Hpstep).
     apply prim_step_exec_inv in Hpstep as (-> & -> & (c & -> & Hstep)).
     iSplitR; auto. eapply step_exec_inv in Hstep; eauto.
+    unfold exec in Hstep.
 
     specialize (indom_regs_incl _ _ _ Dregs Hregs) as Hri. unfold regs_of in Hri.
     destruct (Hri dst) as [wdst [H'dst Hdst]]. by set_solver+.
     destruct (Hri src) as [wsrc [H'src Hsrc]]. by set_solver+.
 
-    rewrite /= /RegLocate Hsrc in Hstep.
-    assert ((c, σ2) = updatePC (update_reg (r, m) dst (WInt (if is_cap wsrc then 1%Z else 0%Z)))) as HH.
-    { unfold is_cap; destruct wsrc; auto. }
+    assert (exec_opt (IsPtr dst src) (r, m) = updatePC (update_reg (r, m) dst (WInt (if is_cap wsrc then 1%Z else 0%Z)))) as HH.
+    {  rewrite /= /RegLocate Hsrc. unfold is_cap; destruct wsrc; auto. }
+    rewrite HH in Hstep. rewrite /update_reg /= in Hstep.
 
     destruct (incrementPC (<[ dst := WInt (if is_cap wsrc then 1%Z else 0%Z) ]> regs))
       as [regs'|] eqn:Hregs'; pose proof Hregs' as H'regs'; cycle 1.
@@ -69,14 +70,15 @@ Section cap_lang_rules.
       2: by apply lookup_insert_is_Some'; eauto.
       2: by apply insert_mono; eauto.
       simplify_pair_eq.
-      iMod ((gen_heap_update_inSepM _ _ dst) with "Hr Hmap") as "[Hr Hmap]"; eauto.
+      rewrite Hregs' in Hstep. inversion Hstep.
       iFrame. iApply "Hφ"; iFrame. iPureIntro. econstructor; eauto. }
 
     (* Success *)
 
     eapply (incrementPC_success_updatePC _ m) in Hregs'
       as (p' & g' & b' & e' & a'' & a_pc' & HPC'' & HuPC & ->).
-    eapply updatePC_success_incl with (m':=m) in HuPC. 2: by eapply insert_mono; eauto.
+    eapply updatePC_success_incl with (m':=m) in HuPC. 2: by eapply insert_mono; eauto. rewrite HuPC in Hstep.
+
     simplify_pair_eq. iFrame.
     iMod ((gen_heap_update_inSepM _ _ dst) with "Hr Hmap") as "[Hr Hmap]"; eauto.
     iMod ((gen_heap_update_inSepM _ _ PC) with "Hr Hmap") as "[Hr Hmap]"; eauto.
