theories/rules/rules_Lea.v
@@ -83,28 +83,18 @@ Section cap_lang_rules.
      iNext. iIntros (e2 σ2 efs Hpstep).
      apply prim_step_exec_inv in Hpstep as (-> & -> & (c & -> & Hstep)).
      iSplitR; auto. eapply step_exec_inv in Hstep; eauto.
+     unfold exec in Hstep; simpl in Hstep.
 
      specialize (indom_regs_incl _ _ _ Dregs Hregs) as Hri. unfold regs_of in Hri.
 
      feed destruct (Hri r1) as [r1v [Hr'1 Hr1]]. by set_solver+.
      pose proof (regs_lookup_eq _ _ _ Hr1) as Hr1'.
-     cbn in Hstep. rewrite Hr1' in Hstep.
-     destruct r1v as [| p b e a ] eqn:Hr1v.
-     { (* Failure: r1 is not a capability *)
-       assert (c = Failed ∧ σ2 = (r, m)) as (-> & ->)
-         by (destruct arg; inversion Hstep; auto).
-       iFailWP "Hφ" Lea_fail_r1_noncap. }
-
-     destruct (perm_eq_dec p E); [ subst p |].
-     { (* Failure: r1.p is Enter *)
-       assert (c = Failed ∧ σ2 = (r, m)) as (-> & ->).
-       { destruct arg; inversion Hstep; subst; eauto. }
-       iFailWP "Hφ" Lea_fail_p_E. }
+     rewrite Hr1' in Hstep.
 
      destruct (z_of_argument regs arg) as [ argz |] eqn:Harg;
        pose proof Harg as Harg'; cycle 1.
      { (* Failure: argument is not a constant (z_of_argument regs arg = None) *)
-       unfold z_of_argument in Harg. destruct arg as [| r0]; [ congruence |].
+       unfold z_of_argument in Harg, Hstep. destruct arg as [| r0]; [ congruence |].
        feed destruct (Hri r0) as [r0v [Hr'0 Hr0]].
        { unfold regs_of_argument. set_solver+. }
        rewrite /RegLocate Hr0 Hr'0 in Harg Hstep.
@@ -112,59 +102,54 @@ Section cap_lang_rules.
        assert (c = Failed ∧ σ2 = (r, m)) as (-> & ->)
          by (destruct p; inversion Hstep; eauto).
        iFailWP "Hφ" Lea_fail_rv_nonconst. }
+    apply (z_of_arg_mono _ r) in Harg. rewrite Harg in Hstep; cbn in Hstep.
+
+
+     destruct r1v as [| p b e a ] eqn:Hr1v.
+     { (* Failure: r1 is not a capability *)
+       inversion Hstep.
+       iFailWP "Hφ" Lea_fail_r1_noncap. }
+
+     destruct (perm_eq_dec p E); [ subst p |].
+     { (* Failure: r1.p is Enter *)
+       inversion Hstep.
+       iFailWP "Hφ" Lea_fail_p_E. }
 
      destruct (a + argz)%a as [ a' |] eqn:Hoffset; cycle 1.
      { (* Failure: offset is too large *)
-       unfold z_of_argument in Harg. destruct arg as [ z | r0].
-       { inversion Harg; subst z. rewrite Hoffset in Hstep.
          assert (c = Failed ∧ σ2 = (r, m)) as (-> & ->)
            by (destruct p; inversion Hstep; auto).
          iFailWP "Hφ" Lea_fail_overflow. }
-       { feed destruct (Hri r0) as [r0v [Hr'0 Hr0]].
-         by unfold regs_of_argument; set_solver+.
-         rewrite /RegLocate Hr'0 Hr0 in Harg Hstep.
-         destruct r0v; [| congruence]. inversion Harg; subst z.
-         rewrite Hoffset in Hstep.
-         assert (c = Failed ∧ σ2 = (r, m)) as (-> & ->)
-           by (destruct p; inversion Hstep; auto).
-         iFailWP "Hφ" Lea_fail_overflow. } }
 
-     assert ((c, σ2) = updatePC (update_reg (r, m) r1 (WCap p b e a'))) as HH.
-     { unfold z_of_argument in Harg. destruct arg as [ z | r0 ].
-       { inversion Harg; subst z. rewrite Hoffset in Hstep.
-         destruct p; auto; try congruence; destruct (Addr_le_dec a' a); try congruence; auto; solve_addr. }
-       { feed destruct (Hri r0) as [r0v [Hr'0 Hr0]].
-         by unfold regs_of_argument; set_solver+.
-         rewrite /RegLocate Hr'0 Hr0 in Harg Hstep.
-         destruct r0v; [| congruence]. inversion Harg; subst z.
-         rewrite Hoffset in Hstep.
-         destruct p; auto; try congruence; destruct (Addr_le_dec a' a); try congruence; auto; solve_addr. } }
-     clear Hstep. rewrite /update_reg /= in HH.
-
+     rewrite /update_reg /= in Hstep.
      destruct (incrementPC (<[ r1 := WCap p b e a' ]> regs)) as [ regs' |] eqn:Hregs';
        pose proof Hregs' as Hregs'2; cycle 1.
      { (* Failure: incrementing PC overflows *)
-       assert (incrementPC (<[ r1 := WCap p b e a' ]> r) = None).
+       assert (incrementPC (<[ r1 := WCap p b e a' ]> r) = None) as HH.
        { eapply incrementPC_overflow_mono; first eapply Hregs'.
          by rewrite lookup_insert_is_Some'; eauto.
          by apply insert_mono; eauto. }
-       rewrite incrementPC_fail_updatePC //= in HH; inversion HH; subst.
-       iMod (@gen_heap_update_inSepM with "Hr Hmap") as "[Hr Hmap]"; eauto.
+       apply (incrementPC_fail_updatePC _ m) in HH. rewrite HH in Hstep.
+       assert (c = Failed ∧ σ2 = (r, m)) as (-> & ->)
+           by (destruct p; inversion Hstep; auto).
        iFailWP "Hφ" Lea_fail_overflow_PC. }
 
      (* Success *)
-
      eapply (incrementPC_success_updatePC _ m) in Hregs'
        as (p' & g' & b' & e' & a'' & a_pc' & HPC'' & HuPC & ->).
      eapply updatePC_success_incl in HuPC. 2: by eapply insert_mono; eauto.
-     rewrite HuPC in HH; clear HuPC; inversion HH; clear HH; subst c σ2. cbn.
+     rewrite HuPC in Hstep; clear HuPC.
+     eassert ((c, σ2) = (NextI, _)) as HH.
+     { destruct p; cbn in Hstep; eauto. congruence. }
+     simplify_pair_eq.
+
      iFrame.
      iMod ((gen_heap_update_inSepM _ _ r1) with "Hr Hmap") as "[Hr Hmap]"; eauto.
      iMod ((gen_heap_update_inSepM _ _ PC) with "Hr Hmap") as "[Hr Hmap]"; eauto.
      iFrame. iModIntro. iApply "Hφ". iFrame. iPureIntro.
      eapply Lea_spec_success; eauto.
 
-     Unshelve. all: assumption.
+     Unshelve. all: auto.
    Qed.
 
    Lemma wp_lea_success_reg_PC Ep pc_p pc_b pc_e pc_a pc_a' w rv z a' :
