theories/rules/rules_Restrict.v
@@ -80,13 +80,11 @@ Section cap_lang_rules.
     iNext. iIntros (e2 σ2 efs Hpstep).
     apply prim_step_exec_inv in Hpstep as (-> & -> & (c & -> & Hstep)).
     iSplitR; auto. eapply step_exec_inv in Hstep; eauto.
+    unfold exec in Hstep. cbn in Hstep.
 
     specialize (indom_regs_incl _ _ _ Dregs Hregs) as Hri.
     unfold regs_of in Hri, Dregs.
     destruct (Hri dst) as [wdst [H'dst Hdst]]. by set_solver+.
-    destruct wdst.
-    { rewrite /= /RegLocate Hdst in Hstep. destruct src; inv Hstep; simplify_pair_eq.
-      all: iFailWP "Hφ" Restrict_fail_dst_noncap. }
 
     destruct (z_of_argument regs src) as [wsrc|] eqn:Hwsrc;
       pose proof Hwsrc as H'wsrc; cycle 1.
@@ -94,41 +92,50 @@ Section cap_lang_rules.
       destruct (Hri r0) as [r0v [Hr'0 Hr0]]. by unfold regs_of_argument; set_solver+.
       rewrite Hr'0 in Hwsrc. destruct r0v; [ congruence |].
       assert (c = Failed ∧ σ2 = (r, m)) as (-> & ->).
-      { rewrite /= /RegLocate Hdst Hr0 in Hstep. by simplify_pair_eq. }
+      { rewrite /= /RegLocate Hdst Hr0 in Hstep. cbn in Hstep. by simplify_pair_eq. }
       iFailWP "Hφ" Restrict_fail_src_nonz. }
-    eapply z_of_argument_Some_inv' in Hwsrc; eauto.
+    apply (z_of_arg_mono _ r) in Hwsrc; auto. rewrite Hwsrc in Hstep; simpl in Hstep.
+
+    destruct wdst.
+    { rewrite /= /RegLocate Hdst in Hstep.  inversion Hstep.
+      all: iFailWP "Hφ" Restrict_fail_dst_noncap. }
+    apply regs_lookup_eq in Hdst. rewrite Hdst in Hstep.
 
     destruct (decide (p = E)).
-    { subst p. cbn in Hstep. rewrite /RegLocate Hdst in Hstep.
-      repeat case_match; inv Hstep; iFailWP "Hφ" Restrict_fail_pE. }
+    { subst p.  inv Hstep.
+       iFailWP "Hφ" Restrict_fail_pE. }
 
     destruct (PermFlowsTo (decodePerm wsrc) p) eqn:Hflows; cycle 1.
-    { rewrite /= /RegLocate Hdst in Hstep.
-      destruct Hwsrc as [ -> | (r0 & -> & Hr0 & Hr0') ].
-      all: rewrite ?Hr0' Hflows in Hstep.
-      all: repeat case_match; inv Hstep; iFailWP "Hφ" Restrict_fail_invalid_perm. }
+    { destruct p; try congruence; inv Hstep ; iFailWP "Hφ" Restrict_fail_invalid_perm. }
 
-    assert ((c, σ2) = updatePC (update_reg (r, m) dst (WCap (decodePerm wsrc) b e a))) as HH.
-    { rewrite /= /RegLocate Hdst in Hstep.
-      destruct Hwsrc as [ -> | (r0 & -> & Hr0 & Hr0') ].
-      all: rewrite ?Hr0' Hflows in Hstep.
-      all: repeat case_match; inv Hstep; eauto; congruence. }
-    clear Hstep. rewrite /update_reg /= in HH.
+    rewrite /update_reg /= in Hstep.
+    (* assert ((c, σ2) = updatePC (update_reg (r, m) dst (WCap (decodePerm wsrc) b e a))) as HH. *)
+    (* { rewrite /= /RegLocate Hdst in Hstep. *)
+    (*   destruct Hwsrc as [ -> | (r0 & -> & Hr0 & Hr0') ]. *)
+    (*   all: rewrite ?Hr0' Hflows in Hstep. *)
+    (*   all: repeat case_match; inv Hstep; eauto; congruence. } *)
+    (* clear Hstep. rewrite /update_reg /= in HH. *)
 
     destruct (incrementPC (<[ dst := WCap (decodePerm wsrc) b e a ]> regs)) eqn:Hregs';
       pose proof Hregs' as H'regs'; cycle 1.
-    { apply incrementPC_fail_updatePC with (m:=m) in Hregs'.
-      eapply updatePC_fail_incl with (m':=m) in Hregs'.
-      2: by apply lookup_insert_is_Some'; eauto.
-      2: by apply insert_mono; eauto.
-      simplify_pair_eq.
-      iMod ((gen_heap_update_inSepM _ _ dst) with "Hr Hmap") as "[Hr Hmap]"; eauto.
+    {
+      assert (incrementPC (<[ dst := WCap( decodePerm wsrc) b e a ]> r) = None) as HH.
+       { eapply incrementPC_overflow_mono; first eapply Hregs'.
+         by rewrite lookup_insert_is_Some'; eauto.
+         by apply insert_mono; eauto. }
+       apply (incrementPC_fail_updatePC _ m) in HH. rewrite HH in Hstep.
+       assert (c = Failed ∧ σ2 = (r, m)) as (-> & ->)
+           by (destruct p; inversion Hstep; auto).
       iFailWP "Hφ" Restrict_fail_PC_overflow. }
 
     eapply (incrementPC_success_updatePC _ m) in Hregs'
       as (p' & g' & b' & e' & a'' & a_pc' & HPC'' & HuPC & ->).
-    eapply updatePC_success_incl with (m':=m) in HuPC. 2: by eapply insert_mono; eauto.
-    simplify_pair_eq. iFrame.
+    eapply updatePC_success_incl with (m':=m) in HuPC. 2: by eapply insert_mono; eauto. rewrite HuPC in Hstep.
+     eassert ((c, σ2) = (NextI, _)) as HH.
+     { destruct p; cbn in Hstep; eauto. congruence. }
+     simplify_pair_eq.
+
+     iFrame.
     iMod ((gen_heap_update_inSepM _ _ dst) with "Hr Hmap") as "[Hr Hmap]"; eauto.
     iMod ((gen_heap_update_inSepM _ _ PC) with "Hr Hmap") as "[Hr Hmap]"; eauto.
     iFrame. iApply "Hφ". iFrame. iPureIntro. econstructor; eauto.
