theories/rules/rules_Subseg.v
@@ -43,7 +43,7 @@ Section cap_lang_rules.
       addr_of_argument regs src2 = Some a2 →
       isWithin a1 a2 b e = true →
       incrementPC (<[ dst := WCap p a1 a2 a ]> regs) = None →
-      Subseg_failure regs dst src1 src2 (<[ dst := WCap p a1 a2 a ]> regs).
+      Subseg_failure regs dst src1 src2 regs.
 
   Inductive Subseg_spec (regs: Reg) (dst: RegName) (src1 src2: Z + RegName) (regs': Reg): cap_lang.val -> Prop :=
   | Subseg_spec_success p b e a a1 a2:
@@ -85,23 +85,16 @@ Section cap_lang_rules.
     iNext. iIntros (e2 σ2 efs Hpstep).
     apply prim_step_exec_inv in Hpstep as (-> & -> & (c & -> & Hstep)).
     iSplitR; auto. eapply step_exec_inv in Hstep; eauto.
+    unfold exec in Hstep; cbn in Hstep.
 
     specialize (indom_regs_incl _ _ _ Dregs Hregs) as Hri.
     unfold regs_of in Hri, Dregs.
     destruct (Hri dst) as [wdst [H'dst Hdst]]. by set_solver+.
-    destruct wdst.
-    { rewrite /= /RegLocate Hdst in Hstep. repeat case_match; inv Hstep; simplify_pair_eq.
-      all: iFailWP "Hφ" Subseg_fail_dst_noncap. }
-
-    destruct (decide (p = E)).
-    { subst p. rewrite /= /RegLocate Hdst in Hstep.
-      repeat case_match; inv Hstep; simplify_pair_eq.
-      all: iFailWP "Hφ" Subseg_fail_pE. }
 
     destruct (addr_of_argument regs src1) as [a1|] eqn:Ha1;
       pose proof Ha1 as H'a1; cycle 1.
-    { destruct src1 as [| r1] eqn:?; cbn in Ha1.
-      { rewrite /= /RegLocate Hdst Ha1 in Hstep.
+    { destruct src1 as [| r1] eqn:?; cbn in Ha1, Hstep.
+      { rewrite /RegLocate Hdst Ha1 /= in Hstep.
         assert (c = Failed ∧ σ2 = (r, m)) as (-> & ->).
         { repeat case_match; inv Hstep; auto. }
         iFailWP "Hφ" Subseg_fail_src1_nonaddr. }
@@ -109,17 +102,19 @@ Section cap_lang_rules.
         by unfold regs_of_argument; set_solver+.
       rewrite /addr_of_argument /= Hr'1 in Ha1.
       assert (c = Failed ∧ σ2 = (r, m)) as (-> & ->).
-      { repeat case_match; simplify_pair_eq.
-        all: rewrite /= /RegLocate Hdst Hr1 ?Ha1 in Hstep.
-        all: repeat case_match; inv Hstep; auto. }
+      { destruct r1v ; simplify_pair_eq.
+        all: unfold addr_of_argument, z_of_argument at 2 in Hstep.
+        all: rewrite /= /RegLocate Hdst Hr1 ?Ha1 /= in Hstep.
+        all: inv Hstep; auto.
+      }
       repeat case_match; try congruence.
       all: iFailWP "Hφ" Subseg_fail_src1_nonaddr. }
-    eapply addr_of_argument_Some_inv' in Ha1 as [z1 [Hz1 Hz1']]; eauto.
+    apply (addr_of_arg_mono _ r) in Ha1; auto. rewrite Ha1 /= in Hstep.
 
     destruct (addr_of_argument regs src2) as [a2|] eqn:Ha2;
       pose proof Ha2 as H'a2; cycle 1.
-    { destruct src2 as [| r2] eqn:?; cbn in Ha2.
-      { rewrite /= /RegLocate Hdst Ha2 in Hstep.
+    { destruct src2 as [| r2] eqn:?; cbn in Ha2, Hstep.
+      { rewrite /RegLocate Hdst Ha2 /= in Hstep.
         assert (c = Failed ∧ σ2 = (r, m)) as (-> & ->).
         { repeat case_match; inv Hstep; auto. }
         iFailWP "Hφ" Subseg_fail_src2_nonaddr. }
@@ -127,41 +122,45 @@ Section cap_lang_rules.
         by unfold regs_of_argument; set_solver+.
       rewrite /addr_of_argument /= Hr'2 in Ha2.
       assert (c = Failed ∧ σ2 = (r, m)) as (-> & ->).
-      { repeat case_match; simplify_pair_eq.
-        all: rewrite /= /RegLocate Hdst Hr2 ?Ha2 in Hstep.
-        all: repeat case_match; inv Hstep; auto. }
+      { destruct r2v ; simplify_pair_eq.
+        all: unfold addr_of_argument, z_of_argument  in Hstep.
+        all: rewrite /= /RegLocate Hdst Hr2 ?Ha2 /= in Hstep.
+        all: inv Hstep; auto.
+      }
       repeat case_match; try congruence.
       all: iFailWP "Hφ" Subseg_fail_src2_nonaddr. }
-    eapply addr_of_argument_Some_inv' in Ha2 as [z2 [Hz2 Hz2']]; eauto.
+    apply (addr_of_arg_mono _ r) in Ha2; auto. rewrite Ha2 /= in Hstep.
 
-    assert ((c, σ2) = if isWithin a1 a2 b e then
-                        updatePC (update_reg (r, m) dst (WCap p a1 a2 a)) else
-                        (Failed, (r, m)))
-      as Hexec.
-    { rewrite -Hstep; clear Hstep. 
-      rewrite /= /RegLocate Hdst.
-      destruct Hz1' as [ -> | [r1 (-> & Hr1 & Hr1') ] ];
-        destruct Hz2' as [ -> | [r2 (-> & Hr2 & Hr2') ] ].
-      all: rewrite ?Hz1 ?Hz2 ?Hr1' ?Hr2'.
-      all: repeat case_match; auto; congruence. }
+    destruct wdst.
+    { rewrite /= /RegLocate Hdst in Hstep. repeat case_match; inv Hstep; simplify_pair_eq.
+      all: iFailWP "Hφ" Subseg_fail_dst_noncap. }
+    apply regs_lookup_eq in Hdst. rewrite Hdst in Hstep.
 
-    clear Hstep.
+    destruct (decide (p = E)).
+    { subst p. inv Hstep.
+      iFailWP "Hφ" Subseg_fail_pE. }
+
+    rewrite /update_reg /= in Hstep.
+
     destruct (isWithin a1 a2 b e) eqn:Hiw; cycle 1.
-    { inv Hexec. iFailWP "Hφ" Subseg_fail_not_iswithin. }
+    { destruct p; try congruence; inv Hstep ; iFailWP "Hφ" Subseg_fail_not_iswithin. }
 
-    destruct (incrementPC (<[ dst := (WCap p a1 a2 a) ]> regs)) eqn:HX;
-      pose proof HX as H'X; cycle 1.
-    { apply incrementPC_fail_updatePC with (m:=m) in HX.
-      eapply updatePC_fail_incl with (m':=m) in HX.
-      2: by apply lookup_insert_is_Some'; eauto.
-      2: by apply insert_mono; eauto.
-      simplify_pair_eq.
-      iMod ((gen_heap_update_inSepM _ _ dst) with "Hr Hmap") as "[Hr Hmap]"; eauto.
-      iFailWP "Hφ" Subseg_fail_incrPC. }
+    destruct (incrementPC (<[ dst := (WCap p a1 a2 a) ]> regs)) eqn:Hregs';
+      pose proof Hregs' as H'regs'; cycle 1.
+    { assert (incrementPC (<[ dst := (WCap p a1 a2 a) ]> r) = None) as HH.
+       { eapply incrementPC_overflow_mono; first eapply Hregs'.
+         by rewrite lookup_insert_is_Some'; eauto.
+         by apply insert_mono; eauto. }
+       apply (incrementPC_fail_updatePC _ m) in HH. rewrite HH in Hstep.
+       assert (c = Failed ∧ σ2 = (r, m)) as (-> & ->)
+           by (destruct p; inversion Hstep; auto).
+       iFailWP "Hφ" Subseg_fail_incrPC. }
 
-    eapply (incrementPC_success_updatePC _ m) in HX
+    eapply (incrementPC_success_updatePC _ m) in Hregs'
       as (p' & g' & b' & e' & a'' & a_pc' & HPC'' & HuPC & ->).
-    eapply updatePC_success_incl with (m':=m) in HuPC. 2: by eapply insert_mono; eauto.
+    eapply updatePC_success_incl with (m':=m) in HuPC. 2: by eapply insert_mono; eauto. rewrite HuPC in Hstep.
+     eassert ((c, σ2) = (NextI, _)) as HH.
+     { destruct p; cbn in Hstep; eauto. congruence. }
     simplify_pair_eq. iFrame.
     iMod ((gen_heap_update_inSepM _ _ dst) with "Hr Hmap") as "[Hr Hmap]"; eauto.
     iMod ((gen_heap_update_inSepM _ _ PC) with "Hr Hmap") as "[Hr Hmap]"; eauto.
